theories/FSets/FMapList.v
@@ -1024,8 +1024,7 @@ Module E := X.
 
 Definition key := E.t.
 
-#[universes(template)]
-Record slist (elt:Type) :=
+Polymorphic Cumulative Record slist (elt:Type) :=
   {this :> Raw.t elt; sorted : sort (@Raw.PX.ltk elt) this}.
 Definition t (elt:Type) : Type := slist elt.
 
